@prefix owl: <http://www.w3.org/2002/07/owl#> .
@prefix rdfs: <http://www.w3.org/2000/01/rdf-schema#> .
@prefix dct: <http://purl.org/dc/terms/> .
@prefix dcat: <http://www.w3.org/ns/dcat#> .
@prefix rdf: <http://www.w3.org/1999/02/22-rdf-syntax-ns#> .
@prefix xsd: <http://www.w3.org/2001/XMLSchema#> .

@prefix ids_int: <https://schema.industrialdataspace.org/interface/> .
@prefix ids_rep: <https://schema.industrialdataspace.org/representation/> .
@prefix ids_mt: <https://schema.industrialdataspace.org/mediaType/> .
@prefix ids_rel: <https://schema.iais.fraunhofer.de/ids/helper/relation/> .

# Classes
# -------

ids_rep:Representation a owl:Class;
    rdfs:label "Representation"@en;
    rdfs:comment "Class of Kind representations, i.e., implementation-focused descriptions using data- and media types or schemas."@en;
    ids_rel:validation [
        ids_rel:forProperty ids_rep:offeredBy;
        ids_rel:relationType ids_rel:OneToMany;
    ].

# Properties
# ----------

ids_rep:mediaType rdfs:subPropertyOf dcat:mediaType;
    a owl:ObjectProperty;
    rdfs:domain ids_rep:Representation;
    rdfs:range ids_mt:MediaType;
    rdfs:label "media type"@en;
    rdfs:comment "The media type of the Representation, as defined by IANA."@en.

ids_rep:conformsToStandard a owl:DatatypeProperty;
    rdfs:domain ids_rep:Representation;
    rdfs:range xsd:anyURI;
    rdfs:label "conformsToStandard"@en;
    rdfs:comment "The standard the Representation conforms to."@en.

ids_rep:schemaLink a owl:DatatypeProperty;
    rdfs:domain ids_rep:Representation;
    rdfs:range xsd:anyURI;
    rdfs:label "schemaLink"@en;
    rdfs:comment "Links to a document that contains additional information like class and type descriptions or integrity constraints describing the Representation's structure."@en.

ids_rep:schemaDefinition a owl:DatatypeProperty;
    rdfs:domain ids_rep:Representation;
    rdfs:range xsd:string;
    rdfs:label "schemaDefinition"@en;
    rdfs:comment "Formal definition of the Representation's structure, matching its data and media type (e.g, JSON Schema or XSD)."@en.

ids_rep:offeredBy a owl:ObjectProperty;
    rdfs:label "offeredBy"@en;
    rdfs:domain ids_rep:Representation;
    rdfs:range ids_int:ServiceInterface;
    rdfs:comment "The interface providing the representation of the DataAsset."@en.
