@prefix owl: <http://www.w3.org/2002/07/owl#> .
@prefix rdfs: <http://www.w3.org/2000/01/rdf-schema#> .
@prefix dct: <http://purl.org/dc/terms/> .
@prefix dcat: <http://www.w3.org/ns/dcat#> .
@prefix rdf: <http://www.w3.org/1999/02/22-rdf-syntax-ns#> .
@prefix xsd: <http://www.w3.org/2001/XMLSchema#> .

@prefix ids_dep: <https://schema.industrialdataspace.org/dataEndpoint/> .
@prefix ids_base: <https://schema.industrialdataspace.org/base/> .
@prefix ids_da: <https://schema.industrialdataspace.org/dataAsset/> .
@prefix ids_prot: <https://schema.industrialdataspace.org/protocolBinding/> .
@prefix ids_contr: <https://schema.industrialdataspace.org/contract/> .
@prefix ids_mt: <https://schema.industrialdataspace.org/mediaType/> .
@prefix ids_dt: <https://schema.industrialdataspace.org/core/parameterDataType/> .
@prefix ids_rel: <https://schema.iais.fraunhofer.de/ids/helper/relation/> .
@prefix ids_doc: <https://schema.iais.fraunhofer.de/ids/helper/documentation/> .
@prefix ids_trans: <https://schema.iais.fraunhofer.de/ids/helper/transformation/> .

# Classes
# -------

ids_dep:DataEndpoint rdfs:subClassOf ids_base:EntityWithLifecycle;
    a owl:Class;
    rdfs:label "DataEndpoint"@en ;
    rdfs:comment "Data Endpoint that may be invoked to retrieve (via service calls, subscription, etc) or push data."@en;
    ids_rel:validation [
        ids_rel:forProperty ids_dep:providedBy;
        ids_rel:constraint ids_rel:NotNull;
    ];
    ids_rel:validation [
        ids_rel:forProperty ids_dep:usagePolicy;
        ids_rel:relationType ids_rel:OneToMany;
    ].

ids_dep:DataService a owl:Class;
    rdfs:label "DataService"@en ;
    rdfs:comment "A certain view or interaction ability on the data provided by a DataEndpoint."@en;
    ids_rel:validation [
        ids_rel:forProperty ids_dep:operation;
        ids_rel:relationType ids_rel:OneToMany;
    ].

ids_dep:Operation a owl:Class;
    ids_trans:isAbstract true;
    rdfs:label "Operation"@en ;
    rdfs:comment "An operation to access a DataService, like the retrieval of a filtered subset of the data."@en;
    ids_rel:validation [
        ids_rel:forProperty ids_dep:opLabel;
        ids_rel:constraint ids_rel:NotNull;
        ids_rel:relationType ids_rel:OneToMany;
    ];
    ids_rel:validation [
        ids_rel:forProperty ids_dep:input;
        ids_rel:relationType ids_rel:OneToMany;
    ];
    ids_rel:validation [
        ids_rel:forProperty ids_dep:output;
        ids_rel:relationType ids_rel:OneToMany;
    ];
    ids_rel:validation [
        ids_rel:forProperty ids_dep:opDescription;
        ids_rel:relationType ids_rel:OneToMany;
    ].

ids_dep:ReqRespOperation rdfs:subClassOf ids_dep:Operation;
    a owl:Class;
    ids_trans:isAbstract true;
    rdfs:label "ReqRespOperation"@en ;
    rdfs:comment "The class of operations following the request/response interaction method."@en.

ids_dep:PubSubOperation rdfs:subClassOf ids_dep:Operation;
    a owl:Class;
    ids_trans:isAbstract true;
    rdfs:label "PubSubOperation"@en ;
    rdfs:comment "The class of operations following the publish/subscribe interaction method."@en.

ids_dep:ReadOperation rdfs:subClassOf ids_dep:ReqRespOperation;
   a owl:Class;
   rdfs:label "ReadOperation"@en ;
   rdfs:comment "An operation to access a DataService in a read-only way (pull)."@en.

ids_dep:WriteOperation rdfs:subClassOf ids_dep:ReqRespOperation;
   a owl:Class;
   rdfs:label "WriteOperation"@en ;
   rdfs:comment "An operation to write data to a DataService (push)."@en.

ids_dep:PublishOperation rdfs:subClassOf ids_dep:PubSubOperation;
   a owl:Class;
   rdfs:label "PublishOperation"@en ;
   rdfs:comment "An operation that publishes data on a DataService for asynchronous retrieval by other clients."@en.

ids_dep:SubscribeOperation rdfs:subClassOf ids_dep:PubSubOperation;
   a owl:Class;
   rdfs:label "SubscribeOperation"@en ;
   rdfs:comment "An operation that enables clients to asynchronously retrieve data that has been published to a DataService."@en.

ids_dep:Parameter a owl:Class;
    rdfs:label "Parameter"@en ;
    rdfs:comment "Specifies how an Operation should be performed."@en;
    ids_rel:validation [
        ids_rel:forProperty ids_dep:paramLabel;
        ids_rel:relationType ids_rel:OneToMany;
    ];
    ids_rel:validation [
        ids_rel:forProperty ids_dep:paramDescription;
        ids_rel:relationType ids_rel:OneToMany;
    ].

ids_dep:InputParameter rdfs:subClassOf ids_dep:Parameter;
    a owl:Class;
    rdfs:label "InputParameter"@en ;
    rdfs:comment "Input Parameter to control an Operation."@en.

ids_dep:OutputParameter rdfs:subClassOf ids_dep:Parameter;
    a owl:Class;
    rdfs:label "OutputParameter"@en ;
    rdfs:comment "Result of an Operation."@en.

ids_dep:Fault rdfs:subClassOf ids_dep:OutputParameter;
    a owl:Class;
    rdfs:label "Fault"@en ;
    rdfs:comment "Result on Operation failure."@en.

ids_dep:Representation a owl:Class;
    rdfs:label "Representation"@en ;
    rdfs:comment "Describes how a Parameter's value is represented."@en.

# Properties for describing a DataEndpoint
# ----------------------------------------

ids_dep:offers a owl:ObjectProperty;
    rdfs:domain ids_dep:DataEndpoint;
    rdfs:range ids_dep:DataService;
    rdfs:label "offers"@en;
    rdfs:comment "A DataService that is offered by the DataEndpoint."@en.

ids_dep:protocolBinding a owl:ObjectProperty;
    rdfs:domain ids_dep:DataEndpoint;
    rdfs:range ids_prot:ProtocolBinding;
    rdfs:label "protocolBinding"@en;
    rdfs:comment "ProtocolBinding to be used for creating access requests to a DataEndpoint using a specific protocol."@en.

ids_dep:providedBy a owl:ObjectProperty;
    rdfs:domain ids_dep:DataEndpoint;
    rdfs:range ids_dep:Connector;
    ids_trans:refByURI true;
    rdfs:label "providedBy"@en;
    rdfs:comment "The Connector that provides this DataEndpoint."@en.

# Properties for describing a DataService
# ---------------------------------------

ids_dep:operation a owl:ObjectProperty;
    rdfs:domain ids_dep:DataService;
    rdfs:range ids_dep:Operation;
    rdfs:label "operation"@en;
    ids_doc:labelPluralForm "operations"@en;
    rdfs:comment "An Operation that can be performed on a DataService."@en.

ids_dep:usagePolicy a owl:ObjectProperty;
    rdfs:domain ids_dep:DataEndpoint;
    rdfs:range ids_contr:ServiceContract;
    rdfs:label "usagePolicy"@en;
    ids_doc:labelPluralForm "usagePolicies"@en;
    rdfs:comment "The ServiceContracts describing usage policies for the DataEndpoint's offerings."@en.

ids_dep:publishes a owl:ObjectProperty;
    rdfs:label "publishes"@en;
    rdfs:domain ids_dep:DataService;
    rdfs:range ids_da:DataAsset;
    rdfs:comment "Data Asset published by the Data Service."@en.


# Properties for describing an Operation
# --------------------------------------

ids_dep:input a owl:ObjectProperty;
    rdfs:domain ids_dep:Operation;
    rdfs:range ids_dep:InputParameter;
    rdfs:label "input"@en;
    ids_doc:labelPluralForm "inputs"@en;
    rdfs:comment "Parameterizes the input of an Operation."@en.

ids_dep:output a owl:ObjectProperty;
    rdfs:domain ids_dep:Operation;
    rdfs:range ids_dep:OutputParameter;
    rdfs:label "output"@en;
    ids_doc:labelPluralForm "outputs"@en;
    rdfs:comment "Holds the result of an Operation."@en.

ids_dep:fault a owl:ObjectProperty;
    rdfs:domain ids_dep:Operation;
    rdfs:range ids_dep:Fault;
    rdfs:label "fault"@en;
    ids_doc:labelPluralForm "faults"@en;
    rdfs:comment "Holds information when an Operation has failed."@en.

ids_dep:opLabel rdfs:subPropertyOf rdfs:label;
    a owl:DatatypeProperty;
    rdfs:domain ids_dep:Operation;
    rdfs:range rdf:PlainLiteral;
    ids_doc:labelPluralForm "opLabels"@en;
    rdfs:label "opLabel"@en;
    rdfs:comment "Freetext label of the Operation as it should be shown in public indexes."@en.

ids_dep:opDescription rdfs:subPropertyOf dct:description;
    a owl:DatatypeProperty;
    rdfs:domain ids_dep:Operation;
    rdfs:range rdf:PlainLiteral;
    ids_doc:labelPluralForm "opDescriptions"@en;
    rdfs:label "opDescription"@en;
    rdfs:comment "Freetext description of the Operation as it should be shown in public indexes."@en.

ids_dep:opFunctionality a owl:DatatypeProperty;
   rdfs:domain ids_dep:Operation;
   rdfs:range xsd:anyURI;
   rdfs:label "opFunctionality"@en;
   rdfs:comment "Links to a description of the functionality the Operation provides, preferably expressed as Linked Data."@en.

ids_dep:opImplementation a owl:DatatypeProperty;
  rdfs:domain ids_dep:Operation;
  rdfs:range xsd:anyURI;
  rdfs:label "opImplementation"@en;
  rdfs:comment "Links to a description about how the operation is implemented. The description should provide information about, e.g., used algorithms, expected preconditions, or assumptions."@en.

# Properties for describing a Parameter
# -------------------------------------

ids_dep:paramLabel rdfs:subPropertyOf rdfs:label;
    a owl:DatatypeProperty;
    rdfs:domain ids_dep:Parameter;
    rdfs:range rdf:PlainLiteral;
    rdfs:label "paramLabel"@en;
    ids_doc:labelPluralForm "paramLabels"@en;
    rdfs:comment "Freetext label of the Parameter as it should be shown in public indexes."@en.

ids_dep:paramName rdfs:subPropertyOf dct:identifier;
    a owl:DatatypeProperty;
    rdfs:domain ids_dep:Parameter;
    rdfs:range xsd:string;
    rdfs:label "paramName"@en;
    rdfs:comment "Name of the Parameter as it must be used in service requests."@en.

ids_dep:paramDescription rdfs:subPropertyOf dct:description;
    a owl:DatatypeProperty;
    rdfs:domain ids_dep:Parameter;
    rdfs:range rdf:PlainLiteral;
    rdfs:label "paramDescription"@en;
    ids_doc:labelPluralForm "paramDescriptions"@en;
    rdfs:comment "Freetext description of the Parameter as it should be shown in public indexes."@en.

ids_dep:semanticType a owl:DatatypeProperty;
    rdfs:domain ids_dep:Parameter;
    rdfs:range xsd:anyURI;
    rdfs:label "semanticType"@en;
    rdfs:comment "Links to a description of the Parameter's semantics, preferably expressed as Linked Data."@en.

ids_dep:representation a owl:ObjectProperty;
    rdfs:domain ids_dep:Parameter;
    rdfs:range ids_dep:Representation;
    rdfs:label "representation"@en;
    rdfs:comment "The Representation of the Parameter's value."@en.

# Properties for describing a Representation
# ------------------------------------------

ids_dep:dataType a owl:ObjectProperty;
    rdfs:domain ids_dep:Representation;
    rdfs:range ids_dt:ParameterDataType;
    rdfs:label "dataType"@en;
    rdfs:comment "Indicates the datatype of the Parameter."@en.

ids_dep:format rdfs:subPropertyOf dct:format;
    a owl:DatatypeProperty;
    rdfs:domain ids_dep:Representation;
    rdfs:range xsd:string;
    rdfs:label "format"@en;
    rdfs:comment "The file format of the Representation. ids_dep:mediaType SHOULD be used if the type of the distribution is defined by IANA."@en.

ids_dep:mediaType rdfs:subPropertyOf dcat:mediaType;
    a owl:ObjectProperty;
    rdfs:domain ids_dep:Representation;
    rdfs:range ids_mt:IANAMediaType;
    rdfs:label "mediaType"@en;
    rdfs:comment "The media type of the Representation, as defined by IANA."@en.

ids_dep:conformsToStandard a owl:DatatypeProperty;
    rdfs:domain ids_dep:Representation;
    rdfs:range xsd:anyURI;
    rdfs:label "conformsToStandard"@en;
    rdfs:comment "The standard the Representation conforms to."@en.

ids_dep:conformsToStructure a owl:DatatypeProperty;
    rdfs:domain ids_dep:Representation;
    rdfs:range xsd:anyURI;
    rdfs:label "conformsToStructure"@en;
    rdfs:comment "Links to a document that contains additional information like class and type descriptions or integrity constraints describing the Representation's structure."@en.

ids_dep:transformationRule a owl:DatatypeProperty;
    rdfs:domain ids_dep:Representation;
    rdfs:range xsd:anyURI;
    rdfs:label "transformationRule"@en;
    rdfs:comment "Links to a document that contains rules or algorithms to transform the Representation into another syntactic format."@en.

ids_dep:volume a owl:DatatypeProperty;
    rdfs:label "volume"@en;
    rdfs:domain ids_dep:Representation;
    rdfs:range xsd:long;
    rdfs:comment "The total uncompressed size of a Representation in MB."@en.