@prefix owl: <http://www.w3.org/2002/07/owl#> .
@prefix rdfs: <http://www.w3.org/2000/01/rdf-schema#> .
@prefix dct: <http://purl.org/dc/terms/> .
@prefix xsd: <http://www.w3.org/2001/XMLSchema#> .
@prefix odrl: <http://www.w3.org/ns/odrl/2/> .
@prefix ids: <https://w3id.org/idsa/core/> .


# Classes
# -------

ids:Action rdfs:subClassOf odrl:Action;
    a owl:Class;
    rdfs:label "Action"@en;
    rdfs:comment "A thing one might be permitted to do or prohibited from doing to something."@en;
.

ids:PxpEndpoint
    a owl:Class;
    rdfs:label "pxp endpoint"@en;
    rdfs:comment "The reference to the endpoint which operates a specific action, URI or reference to an associated PXP interface."@en;
.
# Properties
# ----------

ids:actionRefinement
    a owl:ObjectProperty;
    # rdfs:subPropertyOf odrl:refinement ;
    rdfs:label "action refinement"@en;
    rdfs:domain ids:Action;
    rdfs:range ids:Constraint;
    rdfs:comment "Constraint that refines an Action."@en ;
.

ids:includedIn
    a owl:ObjectProperty;
    rdfs:subPropertyOf odrl:includedIn ;
    rdfs:label "is included in"@en;
    rdfs:domain ids:Action;
    rdfs:range ids:Action;
    rdfs:comment "The subject transitively asserts the object Action."@en ;
.

ids:pxpEndpoint
     a owl:ObjectProperty;
     rdfs:label "has PXP endpoint"@en;
     rdfs:domain ids:Action;
     rdfs:range ids:PxpEndpoint ;
     rdfs:comment "The reference to the endpoint which operates a specific action, URI or reference to an associated PXP interface."@en
.

ids:pxpInterfaceDescription a owl:ObjectProperty;
     rdfs:label "pxp interface description"@en;
     rdfs:domain ids:PxpEndpoint;
     rdfs:range  xsd:anyURI;
     rdfs:comment "The reference to a URI that provides the interface description of a PXP."@en;
.

ids:pxpAccessURI a owl:ObjectProperty;
     rdfs:label "pxp access URI"@en;
     rdfs:domain ids:PxpEndpoint;
     rdfs:range  xsd:anyURI;
     rdfs:comment "The reference to a URI that expresses an exact endpoint of that PXP."@en;
.
