@prefix owl: <http://www.w3.org/2002/07/owl#> .
@prefix rdfs: <http://www.w3.org/2000/01/rdf-schema#> .
@prefix dct: <http://purl.org/dc/terms/> .
@prefix prov: <http://www.w3.org/ns/prov#> .
@prefix xsd: <http://www.w3.org/2001/XMLSchema#> .
@prefix rdf: <http://www.w3.org/1999/02/22-rdf-syntax-ns#> .

@prefix ids_activity: <https://schema.industrialdataspace.org/activity/> .
@prefix ids_rel: <https://schema.iais.fraunhofer.de/ids/helper/relation/> .
@prefix ids_trans: <https://schema.iais.fraunhofer.de/ids/helper/transformation/> .
@prefix ids_doc: <https://schema.iais.fraunhofer.de/ids/helper/documentation/> .

# Classes
# -------

ids_activity:Activity rdfs:subClassOf prov:Activity;
    a owl:Class;
    ids_trans:isAbstract true;
    rdfs:label "Activity"@en ;
    rdfs:comment "Something that occurs over a period of time and acts upon or with entities."@en;
    ids_rel:validation [
        ids_rel:forProperty ids_activity:startedBy;
        ids_rel:constraint ids_rel:NotNull;
    ];
    ids_rel:validation [
        ids_rel:forProperty ids_activity:startedAt;
        ids_rel:constraint ids_rel:NotNull;
    ];
    ids_rel:validation [
        ids_rel:forProperty ids_activity:activityDescription;
        ids_rel:relationType ids_rel:OneToMany;
    ].

ids_activity:CreationActivity rdfs:subClassOf ids_activity:Activity;
    a owl:Class;
    rdfs:label "CreationActivity"@en ;
    rdfs:comment "Activity with the goal to generate or produce an entity."@en.

ids_activity:RemovalActivity rdfs:subClassOf ids_activity:Activity;
    a owl:Class;
    rdfs:label "RemovalActivity"@en ;
    rdfs:comment "Activity with the goal to decommission an entity so that it can never be used anymore."@en.

ids_activity:ProvisioningActivity rdfs:subClassOf ids_activity:Activity;
    a owl:Class;
    rdfs:label "ProvisioningActivity"@en ;
    rdfs:comment "Activity with the goal to bring an entity into an operational state."@en.

ids_activity:ShutdownActivity rdfs:subClassOf ids_activity:Activity;
    a owl:Class;
    rdfs:label "ShutdownActivity"@en ;
    rdfs:comment "Activity with the goal to make an entity unoperational, while retaining it and make it operational again at a later point in time."@en.

ids_activity:PublicationActivity rdfs:subClassOf ids_activity:Activity;
    a owl:Class;
    rdfs:label "PublicationActivity"@en ;
    rdfs:comment "Activity with the goal to make available an entity for public or restricted access."@en.

ids_activity:WithdrawActivity rdfs:subClassOf ids_activity:Activity;
    a owl:Class;
    rdfs:label "WithdrawActivity"@en ;
    rdfs:comment "Activity with the goal to withdraw public or restrict availability of an entity."@en.

ids_activity:SuspensionActivity rdfs:subClassOf ids_activity:Activity;
    a owl:Class;
    rdfs:label "SuspensionActivity"@en ;
    rdfs:comment "Activity with the goal to temporarily suspend operation of an entity."@en.

ids_activity:ResumptionActivity rdfs:subClassOf ids_activity:Activity;
    a owl:Class;
    rdfs:label "ResumptionActivity"@en ;
    rdfs:comment "Activity with the goal to resume operation of a temporarily suspended entity."@en.

# Properties
# ----------

ids_activity:activityDescription rdfs:subPropertyOf dct:description;
    a owl:DatatypeProperty;
    rdfs:domain ids_activity:Activity;
    rdfs:range rdf:PlainLiteral;
    rdfs:label "activityDescription"@en;
    ids_doc:labelPluralForm "activityDescriptions"@en;
    rdfs:comment "Freetext description of what has been performed by the Activity."@en.

ids_activity:startedBy rdfs:subPropertyOf prov:wasStartedBy;
    a owl:ObjectProperty;
    rdfs:domain ids_activity:Activity;
    rdfs:range ids_activity:Participant;
    ids_trans:refByURI true;
    rdfs:label "startedBy"@en;
    rdfs:comment "The participant who started the Activity."@en.

ids_activity:startedAt rdfs:subPropertyOf prov:wasStartedBy;
    a owl:DatatypeProperty;
    rdfs:domain ids_activity:Activity;
    rdfs:range xsd:dateTime;
    rdfs:label "startedAt"@en;
    rdfs:comment "The point in time when the Activity was started."@en.

ids_activity:endedBy rdfs:subPropertyOf prov:wasEndedBy;
    a owl:ObjectProperty;
    rdfs:domain ids_activity:Activity;
    rdfs:range ids_activity:Participant;
    ids_trans:refByURI true;
    rdfs:label "endedBy"@en;
    rdfs:comment "The participant who ended the Activity."@en.

ids_activity:endedAt rdfs:subPropertyOf prov:wasEndedBy;
    a owl:DatatypeProperty;
    rdfs:domain ids_activity:Activity;
    rdfs:range xsd:dateTime;
    rdfs:label "endedAt"@en;
    rdfs:comment "The point in time when the Activity was ended."@en.